chg: Restructured States.v
- Added a predicate `contains`, mainly to improve readability and
  potential refactoring
- Reordered the whole file
- Updated proofs in other files
- Improved names of lemmas

theories/FO/States.v
@@ -3,23 +3,205 @@ From InqLog.FO Require Export Models.
 
 (** * Basic definitions
 
-   We now introduce the notion of a [state] which is just a
-   set of worlds in a model.
+   We now introduce the notion of a [state] which can be seen a set of worlds in a model.
  *)
 
-Print Instances Setoid.
-
-Definition state `{Model} := Morph World bool.
+Definition state `{Model} :=
+  Morph World bool.
 
 (**
-   As we typically just care whether two states behave the
-   same, we introduce this as a relation [state_eq], which
-   is indeed an equivalence relation.
+   We define a predicate [contains] to improve readability.
  *)
-Definition state_eq `{Model} : relation state := Morph_eq.
+Definition contains `{Model} (s : state) (w : World) : Prop :=
+  s w = true.
 
-(** * Example states *)
-(** ** The empty state *)
+Lemma contains_dec `{Model} :
+  forall s w,
+    {contains s w} + {~ contains s w}.
+Proof.
+  intros s w.
+  unfold contains.
+  destruct (s w); [left|right]; congruence.
+Qed.
+
+(** ** Substates
+
+   This section implements the notion of substates in a typical set-theoretic way.
+ *)
+Definition substate `{Model} : relation state :=
+  fun t s =>
+  forall w,
+    contains t w ->
+    contains s w.
+
+(**
+   [substate] is a [PreOrder] which is a [reflexive] and [transitive] [relation], at least, if we follow the way, Coq defines it as such.
+ *)
+Print PreOrder.
+
+Instance substate_PreOrder `{Model} : PreOrder substate.
+Proof.
+  split.
+  -
+    (* Reflexivity *)
+    intros s w H1.
+    exact H1.
+  -
+    (* Transitivity *)
+    intros s1 s2 s3 H1 H2 w H3.
+    auto.
+Qed.
+
+Instance contains_Proper_substate `{Model} :
+  Proper (substate ==> equiv ==> impl) contains.
+Proof.
+  intros t s H1 w1 w2 H2 H3.
+  unfold contains in *.
+  rewrite H2 in H3.
+  apply H1.
+  exact H3.
+Qed.
+
+Lemma substate_contrapos `{Model} :
+  forall s t w,
+    substate t s ->
+    ~ contains s w ->
+    ~ contains t w.
+Proof.
+  intros s t w H1 H2 H3.
+  apply H2.
+  apply H1.
+  exact H3.
+Qed.
+
+(** ** Equivalence/Equality of States
+
+   As we typically just care whether two states behave the same, we introduce this as a relation [state_eq], which is indeed an equivalence relation.
+ *)
+Definition state_eq `{Model} : relation state :=
+  Morph_eq.
+
+(**
+   [contains] respects [state_eq].
+ *)
+Instance contains_Proper `{Model} :
+  Proper (state_eq ==> equiv ==> iff) contains.
+Proof.
+  intros s1 s2 H1 w1 w2 H2.
+  unfold contains.
+  rewrite H1,H2.
+  reflexivity.
+Qed.
+
+(**
+   For every [s : state], [contains s] is a morphism.
+ *)
+Program Definition contains_Morph `{Model} (s : state) : Morph World Prop :=
+  {|
+    morph := contains s
+  |}.
+
+Lemma contains_iff_contains_Morph `{Model} :
+  forall s w,
+    contains s w <->
+    contains_Morph s w.
+Proof.
+  reflexivity.
+Qed.
+
+(**
+   [substate] respects [state_eq].
+ *)
+Instance substate_Proper `{Model} :
+  Proper (state_eq ==> state_eq ==> iff) substate.
+Proof.
+  intros s1 s2 H1 t1 t2 H2.
+  split.
+  all: intros H3 w H4.
+  all: rewrite <- H2 + rewrite H2.
+  all: apply H3.
+  all: rewrite H1 + rewrite <- H1.
+  all: exact H4.
+Qed.
+
+Lemma state_eq_iff_contains `{Model} :
+  forall s1 s2,
+    s1 == s2 <->
+    forall w,
+      contains s1 w <->
+      contains s2 w.
+Proof.
+  intros s1 s2.
+  unfold contains.
+  split.
+  all: intros H1 w.
+  -
+    rewrite H1.
+    reflexivity.
+  -
+    specialize (H1 w).
+    destruct (s1 w),(s2 w).
+    all: intuition.
+Qed.
+
+Lemma state_eq_iff_substate `{Model} :
+  forall s1 s2,
+    state_eq s1 s2 <->
+    substate s1 s2 /\ substate s2 s1.
+Proof.
+  intros s1 s2.
+  split.
+  -
+    intros H1.
+    rewrite H1.
+    split.
+    all: reflexivity.
+  -
+    intros [H1 H2].
+    apply state_eq_iff_contains.
+    intros w.
+    split.
+    all: intros H3.
+    all: rewrite <- H1 + rewrite <- H2.
+    all: exact H3.
+Qed.
+
+(** ** Consistent States
+
+   A state is called _consistent_ if it contains at least one world.
+ *)
+Definition consistent `{Model} (s : state) : Prop :=
+  exists w,
+    contains s w.
+
+(**
+   [consistent] respects [substate].
+ *)
+Instance consistent_Proper_substate `{Model} :
+  Proper (substate ==> impl) consistent.
+Proof.
+  intros s1 s2 H1 [w H2].
+  exists w.
+  rewrite <- H1.
+  exact H2.
+Qed.
+
+(**
+   [consistent] respects [state_eq].
+ *)
+Instance consistent_Proper `{Model} :
+  Proper (state_eq ==> iff) consistent.
+Proof.
+  intros s1 s2 H1.
+  apply state_eq_iff_substate in H1 as [H1 H2].
+  split.
+  all: intros H3.
+  all: rewrite <- H1 + rewrite <- H2.
+  all: exact H3.
+Qed.
+
+(** * Example States *)
+(** ** The Empty State *)
 
 Program Definition empty_state `{Model} : state :=
   {|
@@ -30,7 +212,133 @@ Next Obligation.
   easy.
 Qed.
 
-(** ** Singleton states *)
+Lemma contains_empty_state_E `{Model} :
+  forall w,
+    ~ contains empty_state w.
+Proof.
+  discriminate.
+Qed.
+
+(**
+   [empty_state] is a substate of every state.
+ *)
+Lemma empty_state_substate_I `{Model} :
+  forall t,
+    substate empty_state t.
+Proof.
+  intros t w H1.
+  now apply contains_empty_state_E in H1.
+Qed.
+
+(**
+   The only substate of the empty state is the empty state.
+ *)
+Lemma substate_empty_state_E `{Model} :
+  forall t,
+    substate t empty_state ->
+    t == empty_state.
+Proof.
+  intros t H1.
+  apply state_eq_iff_contains.
+  intros w.
+  split.
+  all: intros H2.
+  -
+    rewrite <- H1.
+    exact H2.
+  -
+    now apply contains_empty_state_E in H2.
+Qed.
+
+(**
+   It it quite obvious that the empty state is the only inconsistent state.
+ *)
+Remark state_eq_empty_state_iff_not_consistent `{Model} :
+  forall s,
+    s == empty_state <->
+    ~ consistent s.
+Proof.
+  intros s.
+  split.
+  -
+    intros H1 [w H2].
+    rewrite H1 in H2.
+    now apply contains_empty_state_E in H2.
+  -
+    intros H1.
+    apply state_eq_iff_contains.
+    intros w.
+    split.
+    all: intros H2.
+    +
+      contradict H1.
+      now exists w.
+    +
+      now apply contains_empty_state_E in H2.
+Qed.
+
+(** ** The Most Inconsistent (nonempty) State *)
+
+Program Definition most_inconsistent `{Model} :
+  state :=
+
+  {|
+    morph := fun _ => true
+  |}.
+
+Next Obligation.
+  repeat intro; reflexivity.
+Qed.
+
+Lemma contains_most_inconsistent_I `{Model} :
+  forall w,
+    contains most_inconsistent w.
+Proof.
+  intros w.
+  reflexivity.
+Qed.
+
+(**
+   Every state is a substate of [most_inconsistent].
+ *)
+Lemma substate_most_inconsistent_I `{Model} :
+  forall t,
+    substate t most_inconsistent.
+Proof.
+  intros t w H1.
+  apply contains_most_inconsistent_I.
+Qed.
+
+(**
+   If [most_inconsistent] is a substate of another state [t], then [t] must be [most_inconsistent].
+ *)
+Lemma most_inconsistent_substate_E `{Model} :
+  forall t,
+    substate most_inconsistent t ->
+    t == most_inconsistent.
+Proof.
+  intros t H1.
+  apply state_eq_iff_contains.
+  intros w.
+  split.
+  all: intros H2.
+  -
+    apply contains_most_inconsistent_I.
+  -
+    rewrite <- H1.
+    exact H2.
+Qed.
+
+Lemma consistent_most_inconsistent_I `{Model} :
+  World ->
+  consistent most_inconsistent.
+Proof.
+  intros w.
+  exists w.
+  apply contains_most_inconsistent_I.
+Qed.
+
+(** ** Singleton States *)
 
 Program Definition singleton `{Model} (w : World) : state :=
   {|
@@ -46,37 +354,126 @@ Next Obligation.
   all: reflexivity + rewrite H1 in H2; contradiction.
 Qed.
 
-Lemma singleton_true `{Model} :
+Lemma contains_singleton_iff `{Model} :
   forall w w',
-    singleton w w' = true <->
+    contains (singleton w) w' <->
     w' == w.
 Proof.
   intros w w'.
-  simpl.
-  unfold "_ ==b _".
+  unfold contains; simpl; unfold "_ ==b _".
   destruct (w' == w) as [H1|H1].
   all: easy.
 Qed.
 
-Lemma singleton_false `{Model} :
+Lemma not_contains_singleton_iff `{Model} :
   forall w w',
-    singleton w w' = false <->
+    ~ contains (singleton w) w' <->
     w' =/= w.
 Proof.
   intros w w'.
   simpl.
-  unfold "_ ==b _".
+  unfold contains; simpl; unfold "_ ==b _".
   destruct (w' == w) as [H1|H1].
   all: easy.
 Qed.
 
-Lemma singleton_refl `{Model} :
+Lemma contains_singleton_refl `{Model} :
   forall w,
-    singleton w w = true.
+    contains (singleton w) w.
 Proof.
   intros w.
-  rewrite singleton_true.
+  rewrite contains_singleton_iff.
   reflexivity.
+Qed.
+
+(**
+   [singleton w] is substate of every state containing [w].
+ *)
+Lemma singleton_substate_iff `{Model} :
+  forall (s : state) w,
+    substate (singleton w) s <->
+    contains s w.
+Proof.
+  intros s w.
+  split.
+  -
+    intros H1.
+    rewrite <- H1.
+    apply contains_singleton_refl.
+  -
+    intros H1 w' H2.
+    apply contains_singleton_iff in H2.
+    rewrite H2.
+    exact H1.
+Qed.
+
+(**
+   If a state is substate of a [singleton] state then it
+   must be the singleton state itself or the empty state.
+ *)
+Lemma substate_singleton_E `{Model} :
+  forall w t,
+    substate t (singleton w) ->
+    (
+      t == empty_state \/
+      t == (singleton w)
+    ).
+Proof.
+  intros w t H1.
+  (**
+     Case distinction whether the world [w] is part of [t]
+     or not.
+   *)
+  destruct (contains_dec t w) as [H2|H2].
+  -
+    right.
+    symmetry.
+    apply state_eq_iff_contains.
+    intros w'.
+    rewrite contains_singleton_iff.
+    split.
+    all: intros H3.
+    +
+      rewrite H3.
+      exact H2.
+    +
+      apply contains_singleton_iff.
+      rewrite <- H1.
+      exact H3.
+  -
+    left.
+    apply state_eq_iff_contains.
+    intros w'.
+    split.
+    all: intros H3.
+    +
+      contradict H2.
+      apply H1 in H3 as H4.
+      apply contains_singleton_iff in H4.
+      rewrite <- H4.
+      exact H3.
+    +
+      now apply contains_empty_state_E in H3.
+Qed.
+
+Instance singleton_Proper `{Model} :
+  Proper (equiv ==> state_eq) singleton.
+Proof.
+  intros w1 w2 H1.
+  apply state_eq_iff_contains.
+  intros w.
+  do 2 rewrite contains_singleton_iff.
+  rewrite H1.
+  reflexivity.
+Qed.
+
+Lemma consistent_singleton_I `{Model} :
+  forall w,
+    consistent (singleton w).
+Proof.
+  intros w.
+  exists w.
+  apply contains_singleton_refl.
 Qed.
 
 (** ** Complement states *)
@@ -92,25 +489,68 @@ Next Obligation.
   reflexivity.
 Qed.
 
-Fact complement_true `{Model} :
+Lemma contains_complement_iff `{Model} :
   forall s w,
-    complement s w = true <->
-    s w = false.
+    contains (complement s) w <->
+    ~ contains s w.
 Proof.
   intros s w.
-  apply negb_true_iff.
+  unfold contains; simpl.
+  rewrite negb_true_iff,not_true_iff_false.
+  reflexivity.
 Qed.
 
-Fact complement_false `{Model} :
+Lemma not_contains_complement_iff `{Model} :
   forall s w,
-    complement s w = false <->
-    s w = true.
+    ~ contains (complement s) w <->
+    contains s w.
 Proof.
   intros s w.
-  apply negb_false_iff.
+  apply eq_true_negb_classical_iff.
 Qed.
 
-Fact complement_complement `{Model} :
+Instance complement_Proper_substate `{Model} :
+  Proper (substate --> substate) complement.
+Proof.
+  intros s1 s2 H1 w H2.
+  apply contains_complement_iff.
+  apply contains_complement_iff in H2.
+  eapply substate_contrapos; eassumption.
+Qed.
+
+(**
+   The [substate] relation turns around for [complement]
+   states.
+ *)
+Lemma complement_substate_complement_iff `{Model} :
+  forall s t,
+    substate (complement s) (complement t) <->
+    substate t s.
+Proof.
+  intros s t.
+  split.
+  -
+    intros w H1 H2.
+    apply not_contains_complement_iff.
+    apply not_contains_complement_iff in H2.
+    eapply substate_contrapos.
+    all: eassumption.
+  -
+    intros H1.
+    rewrite H1.
+    reflexivity.
+Qed.
+
+Instance complement_Proper `{Model} :
+  Proper (state_eq ==> state_eq) complement.
+Proof.
+  intros s1 s2 H1 w.
+  simpl.
+  rewrite H1.
+  reflexivity.
+Qed.
+
+Lemma complement_involutive `{Model} :
   forall s,
     (complement (complement s)) == s.
 Proof.
@@ -118,28 +558,124 @@ Proof.
   apply negb_involutive.
 Qed.
 
-(** ** Mapping states
+(** ** Excluding states
 
-   Mapping states implement the idea that we can describe
-   finite states via (finite) lists of natural numbers and a
-   mapping function.
+   Excluding states implement the idea that we want to be
+   able to exclude a world from a state.
  *)
 
-Program Definition mapping_state
-  `{Model}
-  (f : nat -> World)
-  (ns : list nat) :
-  state :=
-
+Program Definition excluding_state `{Model} (s : state) (w : World) : state :=
   {|
     morph :=
-    fun w =>
-    inbS w (map f ns)
+      fun w' =>
+      if w' == w
+      then false
+      else s w'
+  |}.
+
+Next Obligation.
+  intros w1 w2 H1.
+  destruct (w1 == w) as [H2|H2].
+  all: destruct (w2 == w) as [H3|H3].
+  all: rewrite H1 in *; reflexivity + contradiction.
+Qed.
+
+Lemma contains_excluding_state_iff `{Model} :
+  forall s w w',
+  contains (excluding_state s w) w' <->
+  contains s w' /\
+  w' =/= w.
+Proof.
+  intros s w w'.
+  unfold contains.
+  simpl.
+  split.
+  -
+    intros H1.
+    destruct (w' == w) as [H2|H2]; try discriminate.
+    split.
+    all: assumption.
+  -
+    intros [H1 H2].
+    destruct (w' == w) as [H3|_]; try contradiction.
+    exact H1.
+Qed.
+
+Lemma not_contains_excluding_state_iff `{Model} :
+  forall s w w',
+    ~ contains (excluding_state s w) w' <->
+    ~ contains s w' \/
+    w' == w.
+Proof.
+  intros s w w'.
+  split.
+  -
+    intros H1.
+    destruct (contains_dec s w') as [H2|H2]; try (left; exact H2).
+    destruct (w' == w) as [H3|H3]; try (right; exact H3).
+    exfalso.
+    apply H1.
+    apply contains_excluding_state_iff.
+    split.
+    all: assumption.
+  -
+    intros [H1|H1] H2.
+    all: apply contains_excluding_state_iff in H2 as [H2 H3].
+    all: contradiction.
+Qed.
+
+(**
+   An excluding state is always a substate of its original
+   state.
+ *)
+Lemma excluding_state_substate_I `{Model} :
+  forall s w,
+    substate (excluding_state s w) s.
+Proof.
+  intros s w w' H1.
+  apply contains_excluding_state_iff in H1 as [H1 H2].
+  exact H1.
+Qed.
+
+(**
+   If the original state [s] does not contain a World [w],
+   then excluding [w] from [s] has no effect.
+ *)
+Lemma excluding_state_irrelevance `{Model} :
+  forall (s : state) w,
+    ~ contains s w ->
+    (excluding_state s w) == s.
+Proof.
+  intros s w H1.
+  apply state_eq_iff_contains.
+  intros w'.
+  rewrite contains_excluding_state_iff.
+  split.
+  -
+    now firstorder.
+  -
+    intros H2.
+    split; try assumption.
+    intros H3.
+    rewrite H3 in H2.
+    contradiction.
+Qed.
+
+(** ** Mapping States
+
+   Mapping states implement the idea that we can describe finite states via (finite) lists of natural numbers and a mapping function.
+ *)
+
+Program Definition mapping_state `{Model} (f : nat -> World) (ns : list nat) : state :=
+  {|
+    morph :=
+    flip inbS (map f ns)
   |}.
 
 Next Obligation.
   induction ns as [|n ns' IH].
   all: intros w1 w2 H1.
+  all: unfold flip.
   -
     reflexivity.
   -
@@ -155,25 +691,115 @@ Next Obligation.
     exact H1.
 Qed.
 
-(** [mapping_state] respects [Morph_eq] and [InS_eq]. *)
+Lemma contains_mapping_state_I `{Model} :
+  forall f ns n,
+    InS n ns ->
+    contains (mapping_state f ns) (f n).
+Proof.
+  intros f ns n H1.
+  apply InS_iff_inbS_true.
+  apply InS_map_I.
+  exact H1.
+Qed.
+
+Lemma contains_mapping_state_E `{Model} :
+  forall f ns w,
+    contains (mapping_state f ns) w ->
+    exists n,
+      f n == w /\
+      InS n ns.
+Proof.
+  intros f ns w H1.
+  apply InS_iff_inbS_true in H1.
+  apply InS_map_E in H1.
+  exact H1.
+Qed.
+
+Lemma contains_mapping_state_iff `{Model} :
+  forall f ns w,
+    contains (mapping_state f ns) w <->
+    exists n,
+      f n == w /\
+      InS n ns.
+Proof.
+  intros f ns w.
+  split.
+  -
+    apply contains_mapping_state_E.
+  -
+    intros [n [H1 H2]].
+    rewrite <- H1.
+    apply contains_mapping_state_I.
+    exact H2.
+Qed.
+
+(**
+   [mapping_state] also respects [Morph_eq] and [InS_sublist].
+ *)
+Instance mapping_state_Proper_substate `{Model} :
+  Proper (ext_eq ==> InS_sublist ==> substate) mapping_state.
+Proof.
+  intros f1 f2 H1 ns1 ns2 H2 w H3.
+  apply contains_mapping_state_E in H3 as [n [H3 H4]].
+  specialize (H1 n).
+  rewrite H1 in H3.
+  rewrite <- H3.
+  apply contains_mapping_state_I.
+  apply H2.
+  exact H4.
+Qed.
+
+Lemma substate_mapping_state_E `{Model} :
+  forall f ns t,
+  substate t (mapping_state f ns) ->
+  exists ns',
+    t == (mapping_state f ns') /\
+    InS_sublist ns' ns.
+Proof.
+  intros f ns t H1.
+  exists (filter (fun n => t (f n)) ns).
+  split.
+  -
+    apply state_eq_iff_substate.
+    split.
+    +
+      intros w H2.
+      apply H1 in H2 as H3.
+      apply contains_mapping_state_E in H3 as [n [H3 H4]].
+      rewrite <- H3.
+      apply contains_mapping_state_I.
+      apply InS_filter_I.
+      *
+        rewrite <- H3 in H2.
+        exact H2.
+      *
+        exact H4.
+    +
+      intros w H2.
+      apply contains_mapping_state_E in H2 as [n [H2 H3]].
+      rewrite <- H2.
+      apply InS_filter_E in H3 as [H3 H4].
+      exact H3.
+  -
+    apply filter_InS_sublist_I.
+Qed.
+
+(**
+   [mapping_state] respects [Morph_eq] and [InS_eq].
+ *)
 Instance mapping_state_Proper `{Model} :
   Proper (ext_eq ==> InS_eq ==> state_eq) mapping_state.
 Proof.
-  intros f1 f2 H1 ns1 ns2 H2.
-  intros w.
-  apply InS_iff_inbS.
+  intros f1 f2 H1 ns1 ns2 [H2 H3].
+  apply state_eq_iff_substate.
   split.
-  all: intros H3.
-  all: apply InS_map_E in H3 as [n [H3 H4]].
-  all: rewrite <- H3.
-  all: specialize (H1 n).
-  all: rewrite <- H1 + rewrite H1.
-  all: apply InS_map_I.
-  all: apply H2.
-  all: exact H4.
+
+  all: apply mapping_state_Proper_substate.
+  all: try assumption.
+  symmetry; assumption.
 Qed.
 
-Lemma mapping_state_nil `{Model} :
+Lemma mapping_state_nil_state_eq_empty_state `{Model} :
   forall f,
     (mapping_state f nil) == empty_state.
 Proof.
@@ -181,429 +807,11 @@ Proof.
   reflexivity.
 Qed.
 
-Lemma mapping_state_cons `{Model} :
-  forall f n ns' w,
-    mapping_state f (n :: ns') w =
-    (w ==b (f n)) ||
-    mapping_state f ns' w.
-Proof.
-  intros f n ns' w.
-  reflexivity.
-Qed.
-
-(** ** Excluding states
-
-   Excluding states implement the idea that we want to be
-   able to exclude a world from a state.
- *)
-
-Program Definition excluding_state `{Model} (s : state) (w : World) : state :=
-  {|
-    morph :=
-      fun w' =>
-      if w == w'
-      then false
-      else s w'
-  |}.
-
-Next Obligation.
-  intros w1 w2 H1.
-  destruct (w == w1) as [H2|H2].
-  all: destruct (w == w2) as [H3|H3].
-  all: rewrite H1 in *; reflexivity + contradiction.
-Qed.
-
-(**
-   If the original state [s] does not contain a World [w],
-   then excluding [w] from [s] has no effect.
- *)
-Lemma excluding_state_irrelevance `{Model} :
-  forall (s : state) w,
-    s w = false ->
-    (excluding_state s w) == s.
-Proof.
-  intros s w H1 w'.
-  simpl.
-  destruct (w == w') as [H2|H2].
-  -
-    rewrite H2 in H1.
-    congruence.
-  -
-    reflexivity.
-Qed.
-
-(** * Consistent states
-
-   A state is called _consistent_ if it contains at least
-   one world.
- *)
-Definition consistent `{Model} (s : state) : Prop := exists w, s w = true.
-
-(**
-   It it quite obvious that the empty state is the only
-   inconsistent state.
- *)
-Remark empty_state_not_consistent `{Model} :
-  forall s,
-    s == empty_state <->
-    ~ consistent s.
-Proof.
-  intros s.
-  split.
-  -
-    intros H1 [w H2].
-    rewrite H1 in H2.
-    discriminate.
-  -
-    intros H1 w.
-    destruct (s w) eqn:H2; try reflexivity.
-    exfalso.
-    apply H1.
-    exists w.
-    exact H2.
-Qed.
-
-Fact singleton_consistent `{Model} :
-  forall w,
-    consistent (singleton w).
-Proof.
-  intros w.
-  exists w.
-  apply singleton_true.
-  reflexivity.
-Qed.
-
-Program Definition most_inconsistent `{Model} :
-  state :=
-
-  {|
-    morph := fun _ => true
-  |}.
-
-Next Obligation.
-  repeat intro; reflexivity.
-Qed.
-
-(** * Substates
-
-   This section implements the notion of substates in a
-   typical set-theoretic way.
- *)
-
-Definition substate `{Model} : relation state :=
-  fun t s =>
-  forall w,
-    t w = true -> s w = true.
-
-Lemma substate_contrapos `{Model} :
-  forall s t w,
-    substate t s ->
-    s w = false ->
-    t w = false.
-Proof.
-  intros s t w H1 H2.
-  destruct (t w) eqn:H3; try reflexivity.
-  apply H1 in H3.
-  congruence.
-Qed.
-
-(**
-   We will now see, that [substate] is a [PreOrder].
- *)
-Print PreOrder.
-(**
-   A [PreOrder] is a [reflexive] and [transitive] [relation],
-   at least, if we follow the way, Coq defines it as such.
- *)
-Instance substate_PreOrder `{Model} : PreOrder substate.
-Proof.
-  split.
-  -
-    (* Reflexivity *)
-    intros s w H1.
-    exact H1.
-  -
-    (* Transitivity *)
-    intros s1 s2 s3 H1 H2 w H3.
-    auto.
-Qed.
-
-(**
-   We can also prove that [state_eq] is a congruence relation
-   with respect to [substate]:
- *)
-Instance substate_Proper `{Model} :
-  Proper (state_eq ==> state_eq ==> iff) substate.
-Proof.
-  intros s1 s2 H1 t1 t2 H2.
-  split.
-  all: intros H3 w H4.
-  all: rewrite <- H2 + rewrite H2.
-  all: apply H3.
-  all: rewrite H1 + rewrite <- H1.
-  all: exact H4.
-Qed.
-
-(**
-   The only substate of the empty state is the empty state.
- *)
-Lemma substate_empty_state `{Model} :
-  forall t,
-    substate t empty_state ->
-    t == empty_state.
-Proof.
-  intros t H1 w.
-  destruct (t w) eqn:H2; try reflexivity.
-  apply H1 in H2.
-  discriminate.
-Qed.
-
-(**
-   If a state is substate of a [singleton] state then it
-   must be the singleton state itself or the empty state.
- *)
-Lemma substate_singleton `{Model} :
-  forall w t,
-    substate t (singleton w) ->
-    (
-      t == empty_state \/
-      t == (singleton w)
-    ).
-Proof.
-  intros w t H1.
-  (**
-     Case distinction whether the world [w] is part of [t]
-     or not.
-   *)
-  destruct (t w) eqn:H2.
-  -
-    right.
-    intros w'.
-    destruct (t w') eqn:H3.
-    +
-      symmetry.
-      apply H1.
-      exact H3.
-    +
-      symmetry.
-      apply singleton_false.
-      intros H4.
-      rewrite H4 in H3.
-      congruence.
-  -
-    left.
-    intros w'.
-    destruct (t w') eqn:H3; try reflexivity.
-    apply H1 in H3 as H4.
-    apply singleton_true in H4.
-    rewrite H4 in H3.
-    congruence.
-Qed.
-
-(**
-   [singleton w] is substate of every state containing [w].
- *)
-Lemma singleton_substate `{Model} :
-  forall (s : state) w,
-    s w = true ->
-    substate (singleton w) s.
-Proof.
-  intros s w H1 w' H2.
-  apply singleton_true in H2.
-  rewrite H2.
-  exact H1.
-Qed.
-
-(**
-   The [substate] relation turns around for [complement]
-   states.
- *)
-Lemma substate_complement `{Model} :
-  forall s t,
-    substate t s <->
-    substate (complement s) (complement t).
-Proof.
-  intros s t.
-  split.
-  all: intros H1 w H2.
-  -
-    apply complement_true.
-    apply complement_true in H2.
-    eapply substate_contrapos.
-    all: eassumption.
-  -
-    apply complement_false.
-    apply complement_false in H2.
-    eapply substate_contrapos.
-    all: eassumption.
-Qed.
-
-(**
-   An excluding state is always a substate of its original
-   state.
- *)
-Lemma substate_excluding_state `{Model} :
-  forall s w,
-    substate (excluding_state s w) s.
-Proof.
-  intros s w w' H1.
-  simpl in H1.
-  destruct (w == w') as [H2|H2]; easy.
-Qed.
-
-(**
-   [mapping_state] also respects [Morph_eq] and
-   [InS_sublist].
- *)
-Instance mapping_state_Proper_substate `{Model} :
-  Proper (ext_eq ==> InS_sublist ==> substate) mapping_state.
-Proof.
-  intros f1 f2 H1 ns1 ns2 H2 w H3.
-  apply InS_iff_inbS_true.
-  apply InS_iff_inbS_true in H3.
-  apply InS_map_E in H3 as [n [H3 H4]].
-  rewrite <- H3.
-  specialize (H1 n).
-  rewrite H1.
-  apply InS_map_I.
-  apply H2.
-  exact H4.
-Qed.
-
-Lemma unnamed_helper_States_2 `{Model} :
-  forall t f n ns,
-    substate t (mapping_state f (n :: ns)) ->
-    substate (excluding_state t (f n)) (mapping_state f ns).
-Proof.
-  intros t f n ns H1 w H2.
-  simpl in H2.
-  destruct ((f n) == w) as [H3|H3].
-  -
-    discriminate.
-  -
-    apply H1 in H2 as H4.
-    apply InS_iff_inbS_true.
-    apply InS_iff_inbS_true in H4.
-    simpl in H4.
-    apply InS_cons_E in H4 as [H4|H4].
-    +
-      symmetry in H4.
-      contradiction.
-    +
-      exact H4.
-Qed.
-
-Lemma substate_mapping_state_iff `{Model} :
-  forall f ns t,
-  substate t (mapping_state f ns) <->
-  exists ns',
-    t == (mapping_state f ns') /\
-    InS_sublist ns' ns.
-Proof.
-  intros f ns1 t.
-  split.
-  -
-    intros H1.
-    generalize dependent t.
-    induction ns1 as [|n ns1' IH].
-    all: intros t H1.
-    +
-      exists nil.
-      split.
-      *
-        apply substate_empty_state in H1.
-        rewrite H1, mapping_state_nil.
-        reflexivity.
-      *
-        easy.
-    +
-      destruct (t (f n)) eqn:H2.
-      *
-        specialize IH with
-          (t := excluding_state t (f n)).
-        destruct IH as [ns' [H3 H4]].
-        {
-          apply unnamed_helper_States_2.
-          exact H1.
-        }
-        exists (n :: ns').
-        split.
-        --
-           intros w.
-           rewrite mapping_state_cons.
-           rewrite <- H3.
-           unfold excluding_state.
-           simpl.
-           unfold "_ ==b _".
-           destruct (w == f n) as [H5|H5].
-           ++
-              simpl.
-              rewrite H5.
-              exact H2.
-           ++
-              simpl.
-              destruct (f n == w) as [H6|H6].
-              **
-                 symmetry in H6; contradiction.
-              **
-                 reflexivity.
-        --
-           intros n' H5.
-           apply InS_cons_E in H5 as [H5|H5].
-           ++
-              apply InS_cons_I_hd.
-              exact H5.
-           ++
-              apply InS_cons_I_tl.
-              apply H4.
-              exact H5.
-      *
-        specialize IH with
-          (t := t).
-        destruct IH as [ns' [H3 H4]].
-        {
-          intros w H3.
-          apply H1 in H3 as H4.
-          apply InS_iff_inbS_true in H4.
-          simpl in H4.
-          apply InS_cons_E in H4 as [H4|H4].
-          -
-            rewrite H4 in H3.
-            congruence.
-          -
-            apply InS_iff_inbS_true.
-            exact H4.
-        }
-        exists ns'.
-        split.
-        --
-           exact H3.
-        --
-           apply InS_sublist_cons_I.
-           exact H4.
-  -
-    intros [ns2 [H1 H2]].
-    rewrite H1, H2.
-    reflexivity.
-Qed.
-
-Lemma substate_most_inconsistent `{Model} :
-  forall s,
-    substate s most_inconsistent.
-Proof.
-  intros s w H1.
-  reflexivity.
-Qed.
-
 (** * Restricting a [Model] to a [state] *)
 
 Program Definition restricted_Model `{M : Model} (s : state) : Model :=
   {|
-    World := {w : World | s w = true};
-    World_Setoid :=
-      {|
-        equiv := fun x y => (proj1_sig x == proj1_sig y)%type
-      |};
+    World_Setoid := sig_Setoid (contains_Morph s);
     Individual := Individual;
     Individual_inh := Individual_inh;
     Individual_deceq := Individual_deceq;
@@ -614,35 +822,6 @@ Program Definition restricted_Model `{M : Model} (s : state) : Model :=
       fun w =>
       FInterpretation (proj1_sig w)
  |}.
-
-Next Obligation.
-  (**
-     We need to show tht our new type of [World]s forms a
-     setoid which means that we need to show that its
-     equality relation is indeed an equivalence relation.
-   *)
-  constructor.
-  - (* Reflexivity *)
-    intros x.
-    reflexivity.
-  - (* Symmetry *)
-    intros x y H1.
-    symmetry. exact H1.
-  - (* Transitivity *)
-    intros x y z H1 H2.
-    rewrite H1.
-    exact H2.
-Qed.
-
-Next Obligation.
-  (**
-     In addition, the equality still needs to be decidable
-     which is also easy derivable.
-   *)
-  intros x y.
-  simpl.
-  apply equiv_dec.
-Qed.
 
 Next Obligation.
   (**
@@ -688,151 +867,92 @@ Program Definition restricted_state
 
 Next Obligation.
   intros w1 w2 H1.
-  simpl.
+  red in H1.
   rewrite H1.
   reflexivity.
 Qed.
 
-(**
-   We also need the other direction. For this, we use
-   directly the proof mode as this makes the technical
-   construction more clear.
- *)
-Definition unrestricted_state
-  `{Model}
-  (s : state)
-  (t : @state _ (restricted_Model s)) : state.
+Lemma contains_restricted_state_iff `{Model} :
+  forall s t w,
+    contains (restricted_state s t) w <->
+    contains s (proj1_sig w) /\ contains t (proj1_sig w).
 Proof.
-  unshelve econstructor.
-  - (* Definition of the state *)
-    intros w.
-    destruct (s w) eqn:H1.
-    +
-      exact (t (exist _ _ H1)).
-    +
-      exact false.
-  - (* Prove that this states respect the equality on
-       Worlds. *)
-    intros w1 w2 H1.
-    simpl.
-    (**
-       It is quite interesting to see that we cannot do some
-       easy case distinction whether [w1] is in  [s] or not.
-       For this, it is quite instructive to step inside the
-       proof to look at the proof goal: [s w1] (which would
-       be destructed) appears multiple times. This would
-       lead us to an ill-typed term.
-     *)
-    Fail destruct (s w1).
-    (**
-       We solves this by some sort of generalization.
-     *)
-    set (f :=
-      (
-        fun (b' : bool) (w : World) =>
-        (
-          if b' as b return (s w = b -> bool)
-          then fun H2 : s w = true =>
-            t (exist (fun w : World => s w = true) w H2)
-          else fun _ : s w = false =>
-            false
-        )
-      )
-    ).
-    assert (H42 :
-      forall b1 b2 w1 w2 (H1 : s w1 = b1) (H2 : s w2 = b2),
-        b1 = b2 ->
-        w1 == w2 ->
-        f b1 w1 H1 = f b2 w2 H2
-    ).
-    {
-      clear dependent w1.
-      clear dependent w2.
-      intros b1 b2 w1 w2 H1 H2 H3 H4.
-      destruct b1, b2; try congruence.
-      -
-        apply (@morph_Proper _ _ World_Setoid (eq_setoid bool)).
-        exact H4.
-      -
-        reflexivity.
-    }
-    apply H42.
-    +
-      rewrite H1.
-      reflexivity.
-    +
-      exact H1.
-Defined.
-
-Lemma unnamed_States_helper_1 `{Model} :
-  forall (s t : state) w,
-    s w = false ->
-    unrestricted_state s t w = false.
-Proof.
-  intros s t w H1.
-  unfold unrestricted_state.
+  intros s t w.
+  unfold contains.
   simpl.
-  set (f :=
-    (
-      fun (b' : bool) (w : World) =>
-      (
-        if b' as b return (s w = b -> bool)
-        then fun H2 : s w = true =>
-          t (exist (fun w : World => s w = true) w H2)
-        else fun _ : s w = false =>
-          false
-      )
-    )
-  ).
-  assert (H42 :
-    forall b w H1,
-      b = false ->
-      f b w H1 = false
-  ).
-  {
-    clear dependent w.
-    intros b w H1 H2.
-    unfold f.
-    destruct b; easy.
-  }
-  eapply H42.
-  exact H1.
+  apply andb_true_iff.
 Qed.
 
-Lemma unnamed_States_helper_2 `{Model} :
-  forall (s t : state) w (H1 : s w = true),
-    unrestricted_state s t w = t (exist _ _ H1).
+Program Definition unrestricted_state `{Model} (s : state) (t : @state _ (restricted_Model s)) : state :=
+  {|
+    morph :=
+      fun w =>
+      match contains_dec s w with
+      | left H => t (exist (contains_Morph s) _ H)
+      | right _ => false
+      end
+ |}.
+
+Next Obligation.
+  intros w1 w2 H1.
+  destruct (contains_dec s w1) as [H2|H2].
+  all: destruct (contains_dec s w2) as [H3|H3].
+  -
+    apply sig_eq_lifting with
+      (P := contains_Morph s)
+      (C1 := H2)
+      (C2 := H3)
+      in H1
+      as H4.
+    rewrite H4.
+    reflexivity.
+  -
+    contradict H3.
+    rewrite <- H1.
+    exact H2.
+  -
+    contradict H2.
+    rewrite H1.
+    exact H3.
+  -
+    reflexivity.
+Qed.
+
+Lemma contains_unrestricted_state_iff `{Model} :
+  forall s t w (C1 : contains s w),
+    contains (unrestricted_state s t) w <->
+    contains t (exist (contains_Morph s) _ C1).
 Proof.
-  intros s t w H1.
+  intros s t w C1.
+  unfold contains.
   simpl.
-  set (f :=
-    (
-      fun (b' : bool) (w : World) =>
-      (
-        if b' as b return (s w = b -> bool)
-        then fun H2 : s w = true =>
-          t (exist (fun w : World => s w = true) w H2)
-        else fun _ : s w = false =>
-          false
-      )
-    )
-  ).
-  assert (H42 :
-    forall b w (H1 : s w = b) (H2 : s w = true),
-      f b w H1 = t (exist _ w H2)
-  ).
-  {
-    clear dependent w.
-    intros b w H1 H2.
-    destruct b.
-    -
-      apply (@morph_Proper _ _ World_Setoid (eq_setoid bool)).
-      simpl.
-      reflexivity.
-    -
-      congruence.
-  }
-  apply H42.
+  destruct (contains_dec s w) as [H1|H1].
+  -
+    assert (H2 : w == w) by reflexivity.
+    apply sig_eq_lifting with
+      (P := contains_Morph s)
+      (C1 := C1)
+      (C2 := H1)
+      in H2.
+    rewrite H2.
+    reflexivity.
+  -
+    contradiction.
+Qed.
+
+Lemma not_contains_unrestricted_state_I_domain `{Model} :
+  forall s t w,
+    ~ contains s w ->
+    ~ contains (unrestricted_state s t) w.
+Proof.
+  intros s t w H1 H2.
+  unfold contains in H2.
+  simpl in H2.
+  destruct (contains_dec s w) as [H3|H3].
+  -
+    contradiction.
+  -
+    discriminate.
 Qed.
 
 Lemma unrestricted_substate `{Model} :
@@ -841,24 +961,36 @@ Lemma unrestricted_substate `{Model} :
     substate (unrestricted_state s1 s3) s2.
 Proof.
   intros * H1 w H2.
-  destruct (s1 w) eqn:H3.
+  destruct (contains_dec s1 w) as [H3|H3].
   -
-    rewrite unnamed_States_helper_2 with (H1 := H3) in H2.
+    apply contains_unrestricted_state_iff with (C1 := H3) in H2.
     apply H1 in H2.
-    apply andb_true_iff in H2 as [H21 H22].
+    apply contains_restricted_state_iff in H2 as [H21 H22].
     exact H22.
   -
-    rewrite unnamed_States_helper_1 in H2; easy.
+    apply not_contains_unrestricted_state_I_domain with (t := s3) in H3.
+    contradiction.
 Qed.
 
-Lemma unnamed_States_helper_3 `{Model}:
+Lemma state_eq_restricted_state_unrestricted_state `{Model}:
   forall s t,
     t == (restricted_state s (unrestricted_state s t)).
 Proof.
-  intros s t [w H1].
-  symmetry.
-  simpl.
-  rewrite H1 at 1.
-  simpl.
-  apply unnamed_States_helper_2.
+  intros s t.
+  apply state_eq_iff_contains.
+  intros [w H1].
+  rewrite contains_restricted_state_iff.
+  split.
+  -
+    intros H2.
+    split.
+    +
+      exact H1.
+    +
+      apply contains_unrestricted_state_iff in H2.
+      exact H2.
+  -
+    intros [H2 H3].
+    apply contains_unrestricted_state_iff.
+    exact H3.
 Qed.
